coq/subtyping/decl_properties.v
@@ -1,17 +1,67 @@
+Require Import Coq.Program.Equality.
 Require Import Bool.
 Require Import Metalib.Metatheory.
 Require Import List.
 Require Import subtyping.decl.
 Require Import subtyping.prop_ln.
 
-Notation "T |- j # A <: B" := (d_sub T j A B) (at level 20).
+Notation "Γ |- j # A <: B" := (d_sub Γ j A B) (at level 50, j at level 0, A at next level).
 
-Lemma s_trans : forall Gamma A B C j,
-    d_sub Gamma j A B ->
-    d_sub Gamma j B C ->
-    d_sub Gamma j A C.
-Proof.
-  intros.  
+
+(* Inductive d_sub_size : env -> counter -> typ -> typ -> nat -> Prop :=    (* defn d_sub *)
+ | d_subs__refl : forall (E:env) (A:typ) (n:nat),
+     lc_typ A ->
+     wf_env E ->
+     d_sub_size E counter_z A A n
+ | d_subs__unit : forall (E:env) (n:nat),
+     wf_env E ->
+     d_sub_size E counter_inf typ_unit typ_unit n
+ | d_subs__tvar : forall (E:env) (X:typvar) (n:nat),
+     wf_env E ->
+     d_sub_size E counter_inf (typ_var_f X) (typ_var_f X) n
+ | d_subs__arr1 : forall (E:env) (A1 B1 A2 B2:typ) (n1 n2 : nat),
+     d_sub_size E counter_inf A2 A1 n1 ->
+     d_sub_size E counter_inf B1 B2 n2 ->
+     d_sub_size E counter_inf (typ_arrow A1 B1) (typ_arrow A2 B2) (S (n1 + n2))
+ | d_subs__arr2 : forall (E:env) (c:counter) (A1 B1 A2 B2:typ),
+     d_sub_size E counter_inf A2 A1 ->
+     d_sub_size E c B1 B2 ->
+     d_sub_size E (counter_suc c) (typ_arrow A1 B1) (typ_arrow A2 B2)
+ | d_subs__all : forall (L:vars) (E:env) (A1 A2:typ) (n:nat),
+      ( forall X , X \notin  L  -> d_sub_size  ( X ~ bind_empty  ++  E )  counter_inf  ( open_typ_wrt_typ A1 (typ_var_f X) )   ( open_typ_wrt_typ A2 (typ_var_f X) ) n )  ->
+     d_sub_size E counter_inf (typ_all A1) (typ_all A2)
+ | d_subs__alll1 : forall (L:vars) (E:env) (c:counter) (A B C:typ),
+      ( forall X , X \notin  L  -> d_sub  ( X ~ (bind_typ C)  ++  E )  c  ( open_typ_wrt_typ A (typ_var_f X) )  B )  ->
+     d_sub E (counter_suc c) (typ_all A) B
+ | d_subs__alll2 : forall (L:vars) (E:env) (c:counter) (A B C:typ),
+      ( forall X , X \notin  L  -> d_sub  ( X ~ (bind_typ C)  ++  E )  c  ( open_typ_wrt_typ A (typ_var_f X) )  B )  ->
+     d_sub_size E (counter_tsuc c) (typ_all A) B (S n)
+ | d_subs__varl : forall (E:env) (c:counter) (X:typvar) (A B:typ) (n:nat),
+      binds ( X )  ( (bind_typ B) ) ( E )  ->
+     d_sub_size E c B A n ->
+     d_sub_size E c (typ_var_f X) A (S n)
+ | d_subs__varr : forall (E:env) (c:counter) (A:typ) (X:typvar) (B:typ),
+      binds ( X )  ( (bind_typ B) ) ( E )  ->
+     d_sub_size E c A B ->
+     d_sub_size E c A (typ_var_f X). *)
+
+Lemma s_trans : forall Γ j A B C,
+    d_sub Γ j A B ->
+    d_sub Γ j B C ->
+    d_sub Γ j A C.
+Proof with eauto.
+  intros. generalize dependent A.  generalize dependent C. generalize dependent j. induction B; intros.
+  - dependent destruction H0... 
+    + econstructor... admit.
+  - admit.
+  - dependent destruction H0...
+    + dependent destruction H1...
+      * econstructor. admit.
+      * 
+
+    dependent destruction H1. econstructor... admit.
+    + econstructor... admit.
+
 Admitted.
   
             
